zoo_parabs/pool: [await] → [wait].

lib/examples/fibonacci.ml
@@ -4,6 +4,6 @@ let rec fibonacci n ctx =
   else
     let fut1 = Pool.async ctx (fun ctx -> fibonacci (n - 1) ctx) in
     let fut2 = Pool.async ctx (fun ctx -> fibonacci (n - 2) ctx) in
-    Pool.await ctx fut1 + Pool.await ctx fut2
+    Pool.wait ctx fut1 + Pool.wait ctx fut2
 let fibonacci n pool =
   Pool.run pool (fun ctx -> fibonacci n ctx)
